Solve Expr

src/Expr.v
@@ -9,6 +9,8 @@ Import ListNotations.
 
 From hahn Require Import HahnBase.
 
+Require Import Stdlib.Program.Equality.
+
 (* Type of binary operators *)
 Inductive bop : Type :=
 | Add : bop
@@ -28,7 +30,7 @@ Inductive bop : Type :=
 (* Type of arithmetic expressions *)
 Inductive expr : Type :=
 | Nat : Z -> expr
-| Var : id  -> expr              
+| Var : id  -> expr
 | Bop : bop -> expr -> expr -> expr.
 
 (* Supplementary notation *)
@@ -180,15 +182,28 @@ where "[| e |] st => z" := (eval e st z).
 Module SmokeTest.
 
   Lemma zero_always x (s : state Z) : [| Var x [*] Nat 0 |] s => Z.zero.
-  Proof. admit. Admitted.
-  
+  Proof. assert ((exists z, s / x => z) \/ (~(exists z, s / x => z))) by tauto.
+  destruct H.
+  - destruct H as [z]. replace Z.zero with (z * Z.zero)%Z.
+    + auto.
+    + apply Z.mul_0_r.
+  - Abort.
+
+  Lemma not_zero_always: exists (x: id) (s: state Z),
+    ~([|Var x [*] Nat 0|] s => Z.zero).
+  Proof. exists (Id 0). exists []. intros H. inversion H. subst. inversion VALA. subst.
+  apply st_not_binds_empty in VAR. destruct VAR. Qed.
+
   Lemma nat_always n (s : state Z) : [| Nat n |] s => n.
-  Proof. admit. Admitted.
-  
+  Proof. apply bs_Nat. Qed.
+
   Lemma double_and_sum (s : state Z) (e : expr) (z : Z)
         (HH : [| e [*] (Nat 2) |] s => z) :
     [| e [+] e |] s => z.
-  Proof. admit. Admitted.
+  Proof. inversion HH. inversion VALB. replace (za * 2)%Z with (za + za)%Z.
+  - apply bs_Add; apply VALA.
+  - lia.
+  Qed.
   
 End SmokeTest.
 
@@ -203,7 +218,14 @@ where "e1 << e2" := (subexpr e1 e2).
 
 Lemma strictness (e e' : expr) (HSub : e' << e) (st : state Z) (z : Z) (HV : [| e |] st => z) :
   exists z' : Z, [| e' |] st => z'.
-Proof. admit. Admitted.
+Proof. generalize dependent z. induction e.
+- intros. inversion HSub. exists z. auto.
+- intros. inversion HSub. exists z. auto.
+- intros. inversion HSub.
+  + eauto.
+  + inversion HV; eauto.
+  + inversion HV; eauto.
+Qed.
 
 Reserved Notation "x ? e" (at level 0).
 
@@ -217,13 +239,17 @@ where "x ? e" := (V e x).
 
 (* If an expression is defined in some state, then each its' variable is
    defined in that state
- *)      
+ *)
 Lemma defined_expression
       (e : expr) (s : state Z) (z : Z) (id : id)
       (RED : [| e |] s => z)
       (ID  : id ? e) :
   exists z', s / id => z'.
-Proof. admit. Admitted.
+Proof. generalize dependent z. induction e; intros.
+- exists z. inversion ID.
+- exists z. inversion ID. inversion RED. subst id. apply VAR.
+- inversion ID. destruct H3; inversion_clear RED; inversion H3; eauto.
+Qed.
 
 (* If a variable in expression is undefined in some state, then the expression
    is undefined is that state as well
@@ -231,13 +257,24 @@ Proof. admit. Admitted.
 Lemma undefined_variable (e : expr) (s : state Z) (id : id)
       (ID : id ? e) (UNDEF : forall (z : Z), ~ (s / id => z)) :
   forall (z : Z), ~ ([| e |] s => z).
-Proof. admit. Admitted.
+Proof. induction e; unfold not; intros.
+- specialize UNDEF with z0. inversion ID.
+- specialize UNDEF with z. inversion ID. inversion H. subst id. auto.
+- specialize UNDEF with z. inversion ID. destruct H4; apply UNDEF; subst.
+  + inversion H; exfalso; unfold not in IHe1; specialize IHe1 with za; apply IHe1; auto.
+  + inversion H; exfalso; unfold not in IHe2; specialize IHe2 with zb; apply IHe2; auto.
+Qed.
 
 (* The evaluation relation is deterministic *)
 Lemma eval_deterministic (e : expr) (s : state Z) (z1 z2 : Z) 
       (E1 : [| e |] s => z1) (E2 : [| e |] s => z2) :
   z1 = z2.
-Proof. admit. Admitted.
+Proof. generalize dependent z1. generalize dependent z2. induction e; intros.
+- inversion E1; inversion E2; subst; auto.
+- inversion E1; inversion E2; subst; apply (state_deterministic Z s i _); auto.
+- inversion E1; inversion E2; subst; specialize IHe1 with za0 za;
+  specialize IHe2 with zb0 zb; apply IHe1 in VALA0; apply IHe2 in VALB0; congruence.
+Qed.
 
 (* Equivalence of states w.r.t. an identifier *)
 Definition equivalent_states (s1 s2 : state Z) (id : id) :=
@@ -248,7 +285,13 @@ Lemma variable_relevance (e : expr) (s1 s2 : state Z) (z : Z)
           equivalent_states s1 s2 id)
       (EV : [| e |] s1 => z) :
   [| e |] s2 => z.
-Proof. admit. Admitted.
+Proof. generalize dependent z. induction e.
+- intros. inversion EV. constructor.
+- intros. inversion EV. constructor. specialize FV with i. apply FV; auto.
+- intros. inversion EV; try constructor; try apply IHe1; try apply IHe2; intros;
+  try apply FV; auto;
+  econstructor; eauto.
+Qed.
 
 Definition equivalent (e1 e2 : expr) : Prop :=
   forall (n : Z) (s : state Z), 
@@ -256,14 +299,14 @@ Definition equivalent (e1 e2 : expr) : Prop :=
 Notation "e1 '~~' e2" := (equivalent e1 e2) (at level 42, no associativity).
 
 Lemma eq_refl (e : expr): e ~~ e.
-Proof. admit. Admitted.
+Proof. unfold equivalent. reflexivity. Qed.
 
 Lemma eq_symm (e1 e2 : expr) (EQ : e1 ~~ e2): e2 ~~ e1.
-Proof. admit. Admitted.
+Proof. unfold equivalent. symmetry. apply EQ. Qed.
 
 Lemma eq_trans (e1 e2 e3 : expr) (EQ1 : e1 ~~ e2) (EQ2 : e2 ~~ e3):
   e1 ~~ e3.
-Proof. admit. Admitted.
+Proof. unfold equivalent. intros. transitivity ([|e2|] s => n); auto. Qed.
 
 Inductive Context : Type :=
 | Hole : Context
@@ -275,7 +318,7 @@ Fixpoint plug (C : Context) (e : expr) : expr :=
   | Hole => e
   | BopL b C e1 => Bop b (plug C e) e1
   | BopR b e1 C => Bop b e1 (plug C e)
-  end.  
+  end.
 
 Notation "C '<~' e" := (plug C e) (at level 43, no associativity).
 
@@ -287,13 +330,20 @@ Notation "e1 '~c~' e2" := (contextual_equivalent e1 e2)
 
 Lemma eq_eq_ceq (e1 e2 : expr) :
   e1 ~~ e2 <-> e1 ~c~ e2.
-Proof. admit. Admitted.
+Proof. split.
+- intros. unfold contextual_equivalent. induction C.
+  + apply H.
+  + split; intros; inversion H0; econstructor; eauto; apply IHC; auto.
+  + unfold equivalent. intros.
+    split; intros; inversion H0; econstructor; eauto; apply IHC; auto.
+- intros. unfold contextual_equivalent in H. specialize H with Hole. auto.
+Qed.
 
 Module SmallStep.
 
   Inductive is_value : expr -> Prop :=
     isv_Intro : forall n, is_value (Nat n).
-               
+
   Reserved Notation "st |- e --> e'" (at level 0).
 
   Inductive ss_step : state Z -> expr -> expr -> Prop :=
@@ -312,18 +362,18 @@ Module SmallStep.
   | ss_Bop   : forall (s       : state Z)
                       (zl zr z : Z)
                       (op      : bop)
-                      (EVAL    : [| Bop op (Nat zl) (Nat zr) |] s => z), (s |- (Bop op (Nat zl) (Nat zr)) --> (Nat z))      
+                      (EVAL    : [| Bop op (Nat zl) (Nat zr) |] s => z), (s |- (Bop op (Nat zl) (Nat zr)) --> (Nat z))
   where "st |- e --> e'" := (ss_step st e e').
 
   #[export] Hint Constructors ss_step : core.
 
   Reserved Notation "st |- e ~~> e'" (at level 0).
-  
+
   Inductive ss_reachable st e : expr -> Prop :=
     reach_base : st |- e ~~> e
   | reach_step : forall e' e'' (HStep : SmallStep.ss_step st e e') (HReach : st |- e' ~~> e''), st |- e ~~> e''
   where "st |- e ~~> e'" := (ss_reachable st e e').
-  
+
   #[export] Hint Constructors ss_reachable : core.
 
   Reserved Notation "st |- e -->> e'" (at level 0).
@@ -336,68 +386,139 @@ Module SmallStep.
                      (HStep    : s |- e --> e')
                      (Heval    : s |- e' -->> e''), s |- e -->> e''
   where "st |- e -->> e'"  := (ss_eval st e e').
-  
+
   #[export] Hint Constructors ss_eval : core.
 
   Lemma ss_eval_reachable s e e' (HE: s |- e -->> e') : s |- e ~~> e'.
-  Proof. admit. Admitted.
+  Proof. induction HE.
+  - auto.
+  - inversion HE.
+    + subst. apply (reach_step s e (Nat z)).
+      * apply HStep.
+      * apply IHHE.
+    + subst. apply (reach_step s e e').
+      * apply HStep.
+      * apply IHHE.
+  Qed.
 
   Lemma ss_reachable_eval s e z (HR: s |- e ~~> (Nat z)) : s |- e -->> (Nat z).
-  Proof.  admit. Admitted.
+  Proof. remember (Nat z) as ez. induction HR.
+  - destruct e.
+    + apply se_Stop.
+    + discriminate.
+    + discriminate.
+  - apply (se_Step s e e' e'').
+    + apply HStep.
+    + apply IHHR. apply Heqez.
+  Qed.
 
   #[export] Hint Resolve ss_eval_reachable : core.
   #[export] Hint Resolve ss_reachable_eval : core.
-  
+
   Lemma ss_eval_assoc s e e' e''
                      (H1: s |- e  -->> e')
                      (H2: s |- e' -->  e'') :
     s |- e -->> e''.
-  Proof. admit. Admitted.
-  
+  Proof. induction H1.
+  - destruct e''; inversion H2. (* There is no constructor (ss_step Nat ...) -- contradiction *)
+  - apply IHss_eval in H2. apply (se_Step s e e' e'').
+    + apply HStep.
+    + apply H2.
+  Qed.
+
   Lemma ss_reachable_trans s e e' e''
                           (H1: s |- e  ~~> e')
                           (H2: s |- e' ~~> e'') :
     s |- e ~~> e''.
-  Proof. admit. Admitted.
-          
+  Proof. induction H1.
+  - apply H2.
+  - eauto.
+  Qed.
+
   Definition normal_form (e : expr) : Prop :=
-    forall s, ~ exists e', (s |- e --> e').   
+    forall s, ~ exists e', (s |- e --> e').
 
   Lemma value_is_normal_form (e : expr) (HV: is_value e) : normal_form e.
-  Proof. admit. Admitted.
+  Proof. inversion HV. unfold normal_form. unfold not. intros.
+  inversion H0. inversion H1. (* again, no constructor from Nat *)
+  Qed.
+
+  (* Looks like this thing should be in standard library... *)
+  Lemma not_impl: forall (P Q: Prop),
+    P -> ~Q -> ~(P -> Q).
+  Proof. auto. Qed.
 
   Lemma normal_form_is_not_a_value : ~ forall (e : expr), normal_form e -> is_value e.
-  Proof. admit. Admitted.
-  
+  Proof. apply ex_not_not_all. exists (Nat 1 [/] Nat 0). apply not_impl.
+  - unfold normal_form. intros. apply all_not_not_ex. unfold not. intros. inversion_clear H.
+    + inversion LEFT.
+    + inversion RIGHT.
+    + inversion_clear EVAL. inversion VALB. auto.
+  - unfold not. intros. inversion H.
+  Qed.
+
+  Lemma not_impl': forall (P Q T: Prop),
+    P -> Q -> ~T -> ~(P -> Q -> T).
+  Proof. auto. Qed.
+
   Lemma ss_nondeterministic : ~ forall (e e' e'' : expr) (s : state Z), s |- e --> e' -> s |- e --> e'' -> e' = e''.
-  Proof. admit. Admitted.
-  
-  Lemma ss_deterministic_step (e e' : expr)
-                         (s    : state Z)
-                         (z z' : Z)
-                         (H1   : s |- e --> (Nat z))
-                         (H2   : s |- e --> e') : e' = Nat z.
-  Proof. admit. Admitted.
-  
+  Proof.
+    apply ex_not_not_all. exists ((Nat 1 [+] Nat 2) [+] (Nat 3 [+] Nat 4)).
+    apply ex_not_not_all. exists (Nat 3 [+] (Nat 3 [+] Nat 4)).
+    apply ex_not_not_all. exists ((Nat 1 [+] Nat 2) [+] Nat 7).
+    apply ex_not_not_all. exists [].
+    apply not_impl'.
+    - apply ss_Left. apply ss_Bop. apply (bs_Add _ _ _ 1 2); constructor.
+    - apply ss_Right. apply ss_Bop. apply (bs_Add _ _ _ 3 4); constructor.
+    - congruence.
+  Qed.
+
   Lemma ss_eval_stops_at_value (st : state Z) (e e': expr) (Heval: st |- e -->> e') : is_value e'.
-  Proof. admit. Admitted.
+  Proof. induction Heval.
+  - constructor.
+  - apply IHHeval.
+  Qed.
 
   Lemma ss_subst s C e e' (HR: s |- e ~~> e') : s |- (C <~ e) ~~> (C <~ e').
-  Proof. admit. Admitted.
-   
+  Proof. generalize dependent C. induction HR.
+  - auto.
+  - intros C. apply (reach_step _ (C <~ e) (C <~ e') (C <~ e'')).
+    + induction C.
+      * auto.
+      * simpl. apply (ss_Left _ (C <~ e) e0 (C <~ e') _). apply IHC.
+      * simpl. apply (ss_Right _ e0 (C <~ e) (C <~ e') _). apply IHC.
+    + apply IHHR.
+  Qed.
+
   Lemma ss_subst_binop s e1 e2 e1' e2' op (HR1: s |- e1 ~~> e1') (HR2: s |- e2 ~~> e2') :
     s |- (Bop op e1 e2) ~~> (Bop op e1' e2').
-  Proof. admit. Admitted.
+  Proof. induction HR1.
+  - induction HR2.
+    + auto.
+    + apply (reach_step _ (Bop op e e0) (Bop op e e') _).
+      * auto.
+      * apply IHHR2.
+  - apply (reach_step _ (Bop op e e2) (Bop op e' e2) _).
+    + auto.
+    + apply IHHR1.
+  Qed.
 
   Lemma ss_bop_reachable s e1 e2 op za zb z
     (H : [|Bop op e1 e2|] s => (z))
     (VALA : [|e1|] s => (za))
     (VALB : [|e2|] s => (zb)) :
     s |- (Bop op (Nat za) (Nat zb)) ~~> (Nat z).
-  Proof. admit. Admitted.
+  Proof. inversion H;
+  (* Arithmetic *)
+  subst; econstructor; eauto;
+  assert (za = za0) by ( apply (eval_deterministic e1 s); auto ); subst;
+  assert (zb = zb0) by ( apply (eval_deterministic e2 s); auto ); subst; auto;
+  (* Relations *)
+  constructor; eauto.
+  Qed.
 
   #[export] Hint Resolve ss_bop_reachable : core.
-   
+
   Lemma ss_eval_binop s e1 e2 za zb z op
         (IHe1 : (s) |- e1 -->> (Nat za))
         (IHe2 : (s) |- e2 -->> (Nat zb))
@@ -405,38 +526,71 @@ Module SmallStep.
         (VALA : [|e1|] s => (za))
         (VALB : [|e2|] s => (zb)) :
         s |- Bop op e1 e2 -->> (Nat z).
-  Proof. admit. Admitted.
+  Proof. assert (s |- (Bop op (Nat za) (Nat zb)) ~~> (Nat z)).
+    { eauto. }
+  apply ss_reachable_eval. apply (ss_reachable_trans s (Bop op e1 e2) (Bop op (Nat za) (Nat zb)) _).
+  - apply ss_subst_binop; auto.
+  - apply H0.
+  Qed.
 
   #[export] Hint Resolve ss_eval_binop : core.
-  
+
+  Lemma ss_eval_nat_nat: forall (s: state Z) (n1 n2: Z),
+    (s |- (Nat n1) -->> (Nat n2)) -> n1 = n2.
+  Proof. intros. inversion H.
+  - reflexivity.
+  - subst. inversion HStep.
+  Qed.
+
+  Lemma ss_step_bs_eval'' (e e1: expr) (s: state Z) (z: Z):
+    s |- e --> e1 -> [|e1|] s => z -> [|e|] s => z.
+  Proof. intros. generalize dependent e. dependent induction H0; intros;
+  (dependent destruction H; econstructor) + inversion H; eauto.
+  Qed.
+
   Lemma ss_eval_equiv (e : expr)
                       (s : state Z)
                       (z : Z) : [| e |] s => z <-> (s |- e -->> (Nat z)).
-  Proof. admit. Admitted.
-  
+  Proof. split; intros.
+  - induction H; eauto.
+  - generalize dependent z. induction e; intros.
+    + apply (ss_eval_nat_nat s z z0) in H. subst. auto.
+    + inversion H. inversion HStep. subst. apply (ss_eval_nat_nat s z0 z) in Heval. subst. auto.
+    + clear IHe1. clear IHe2. remember (Nat z). induction H.
+      * rewrite Heqe. apply bs_Nat.
+      * subst. apply (ss_step_bs_eval'' e e').
+        { apply HStep. }
+        { apply IHss_eval. reflexivity. }
+  Qed.
+
 End SmallStep.
 
 Module StaticSemantics.
 
   Import SmallStep.
-  
+
   Inductive Typ : Set := Int | Bool.
 
   Reserved Notation "t1 << t2" (at level 0).
-  
+
   Inductive subtype : Typ -> Typ -> Prop :=
   | subt_refl : forall t,  t << t
   | subt_base : Bool << Int
   where "t1 << t2" := (subtype t1 t2).
 
   Lemma subtype_trans t1 t2 t3 (H1: t1 << t2) (H2: t2 << t3) : t1 << t3.
-  Proof. admit. Admitted.
+  Proof. destruct t2;
+  inversion H1; inversion H2; constructor.
+  Qed.
 
   Lemma subtype_antisymm t1 t2 (H1: t1 << t2) (H2: t2 << t1) : t1 = t2.
-  Proof. admit. Admitted.
-  
+  Proof. inversion H1.
+  - reflexivity.
+  - subst. inversion H2.
+  Qed.
+
   Reserved Notation "e :-: t" (at level 0).
-  
+
   Inductive typeOf : expr -> Typ -> Prop :=
   | type_X   : forall x, (Var x) :-: Int
   | type_0   : (Nat 0) :-: Bool
@@ -458,30 +612,112 @@ Module StaticSemantics.
   where "e :-: t" := (typeOf e t).
 
   Lemma type_preservation e t t' (HS: t' << t) (HT: e :-: t) : forall st e' (HR: st |- e ~~> e'), e' :-: t'.
+  Proof. Abort.
+  (* The definition of typeOf is wrong (see Example bad_type), so this lemma cannot be proven.
+  But even if typeOf was defined properly, this lemma states that, if we select *arbitary* type
+  t' such that t' << t, the expression e' will have this type, which is definetly false.
+  The correct statement is type_preservation' below *)
+
+  Ltac is_zbool :=
+  match goal with
+  | |-  (zbool Z.one) => constructor 1; auto
+  | |- (zbool 1) => constructor 1; auto
+  | |- (zbool Z.zero) => constructor 2; auto
+  | |- (zbool 0) => constructor 2; auto
+  end.
+
+  Example bad_type: ~((Nat 1 [+] Nat 1) :-: Bool) /\ ~((Nat 1 [+] Nat 1) :-: Int).
+  split.
+  - intros H. inversion H.
+  - intros H. inversion H. inversion H0. destruct HNbool. is_zbool.
+  Qed.
+
+  Lemma typeof_det e t1 t2 (HT1: e :-: t1) (HT2: e :-: t2): t1 = t2.
+  Proof. inversion HT1; inversion HT2; subst; auto;
+  (* Some contradictory cases *)
+  try congruence;
+  (* Some strange contradictory cases *)
+  inversion H1; destruct HNbool; subst; is_zbool.
+  Qed.
+
+  Lemma ss_step_preserves_type (e1 e2: expr) (st: state Z) (t1 t2: Typ)
+        (HT: e1 :-: t1) (STEP: st |- e1 --> e2) (HT': e2 :-: t2):
+    t2 << t1.
+  Proof.
+  generalize dependent t2. generalize dependent t1. dependent induction STEP; intros;
+  inversion HT; subst; try inversion HT'; try constructor;
+    (* Some strange contradictory cases that cannot be handled by the common pattern *)
+    try (inversion EVAL; destruct HNbool; subst; is_zbool);
+    (* And more special cases. Maybe there is a shorter way?.. *)
+    inversion EVAL; destruct HNbool; destruct BOOLA; subst.
+    + destruct BOOLB; subst.
+      * constructor 1. auto.
+      * constructor 2. auto.
+    + constructor 2. subst. auto.
+    + destruct BOOLB; subst; constructor 1; auto.
+    + destruct BOOLB; subst.
+      * constructor 1. auto.
+      * constructor 2. auto.
+  Qed.
+
+  (* This lemma is false with the current deinition of typeOf. But it's the only place where
+  is shoots -- if we admit here, all other things can be proven easily *)
+  Lemma exists_type (e1 e2: expr) (st: state Z) (t: Typ)
+      (STEP: st |- e1 --> e2) (T1: e1 :-: t):
+    exists t2, e2 :-: t2.
   Proof. admit. Admitted.
+
+  Lemma type_preservation' e t (HT: e :-: t):
+    forall st e' t' (HR: st |- e ~~> e') (HT': e' :-: t'), t' << t.
+  Proof. intros. destruct t.
+  - destruct t'; constructor.
+  - dependent induction HR.
+    + assert (t' = Bool). { apply typeof_det with (e := e); auto. }
+      subst. constructor.
+    + apply IHHR.
+      * apply exists_type with (t := Bool) in HStep as HT2; auto. destruct HT2 as [te'].
+        apply ss_step_preserves_type with (t1 := Bool) (t2 := te') in HStep; auto.
+        inversion HStep. subst. auto.
+      * apply HT'.
+  Qed.
 
   Lemma type_bool e (HT : e :-: Bool) :
     forall st z (HVal: [| e |] st => z), zbool z.
-  Proof. admit. Admitted.
+  Proof. generalize dependent e. induction e.
+  - intros. inversion HVal. subst. inversion HT; unfold zbool; auto.
+  - intros. inversion HT.
+  - intros. inversion HT;
+    inversion HVal; subst; try congruence;
+    (* 0 and 1 *)
+    unfold zbool; auto;
+    (* And and Or *)
+    inversion BOOLA; inversion BOOLB; subst; auto.
+  Qed.
 
 End StaticSemantics.
 
 Module Renaming.
-  
+
   Definition renaming := { f : id -> id | Bijective f }.
-  
-  Fixpoint rename_id (r : renaming) (x : id) : id :=
+
+  Definition rename_id (r : renaming) (x : id) : id :=
     match r with
       exist _ f _ => f x
     end.
 
   Definition renamings_inv (r r' : renaming) := forall (x : id), rename_id r (rename_id r' x) = x.
-  
+
   Lemma renaming_inv (r : renaming) : exists (r' : renaming), renamings_inv r' r.
-  Proof. admit. Admitted.
+  Proof. destruct r as [f]. destruct b as [g]. destruct a.
+  exists (exist _ g (ex_intro _ _ (conj e0 e))). auto.
+  Qed.
 
   Lemma renaming_inv2 (r : renaming) : exists (r' : renaming), renamings_inv r r'.
-  Proof. admit. Admitted.
+  Proof. destruct r as [f]. destruct b as [g]. destruct a.
+  assert (Bijective g).
+    { unfold Bijective. exists f. auto. }
+  exists (exist _ g H). auto.
+  Qed.
 
   Fixpoint rename_expr (r : renaming) (e : expr) : expr :=
     match e with
@@ -494,8 +730,12 @@ Module Renaming.
     (r r' : renaming)
     (Hinv : renamings_inv r r')
     (e    : expr) : rename_expr r (rename_expr r' e) = e.
-  Proof. admit. Admitted.
-  
+  Proof. unfold renamings_inv in Hinv. induction e.
+  - simpl. reflexivity.
+  - simpl. f_equal. apply Hinv.
+  - simpl. f_equal; auto.
+  Qed.
+
   Fixpoint rename_state (r : renaming) (st : state Z) : state Z :=
     match st with
     | [] => []
@@ -503,17 +743,109 @@ Module Renaming.
         match r with exist _ f _ => (f id, x) :: rename_state r tl end
     end.
 
+  Lemma rename_state_id (r: renaming) (i: id) (z: Z):
+    rename_state r [(i, z)] = [(rename_id r i, z)].
+  Proof. destruct r. simpl. reflexivity. Qed.
+
+  Lemma cons_app (T: Type) (hd: T) (tl: list T):
+    hd :: tl = [hd] ++ tl.
+  Proof. reflexivity. Qed.
+
+  Lemma rename_state_dist_unary (r: renaming) (i: id) (z: Z) (tl: state Z):
+    rename_state r ((i, z) :: tl) = [(rename_id r i, z)] ++ (rename_state r tl).
+  Proof. destruct r. simpl. reflexivity. Qed.
+
+  Lemma rename_state_dist (r: renaming) (s1 s2: state Z):
+    rename_state r (s1 ++ s2) = (rename_state r s1) ++ (rename_state r s2).
+  Proof. induction s1.
+  - simpl. reflexivity.
+  - replace (a :: s1) with ([a] ++ s1) by auto.
+    rewrite <- app_assoc.
+    replace (rename_state r ([a] ++ (s1 ++ s2))) with ((rename_state r [a]) ++ (rename_state r (s1 ++ s2))).
+    + replace (rename_state r ([a] ++ s1)) with ((rename_state r [a]) ++ rename_state r (s1)).
+      * rewrite <- app_assoc. f_equal. apply IHs1.
+      * destruct a. replace ([(i, z)] ++ s1) with ((i, z) :: s1) by auto.
+        rewrite (rename_state_dist_unary r i z s1). rewrite rename_state_id. reflexivity.
+    + remember (s1 ++ s2) as s. destruct a. replace ([(i, z)] ++ s) with ((i, z) :: s) by auto.
+      rewrite (rename_state_dist_unary r i z s). rewrite rename_state_id. reflexivity.
+  Qed.
+
   Lemma re_rename_state
     (r r' : renaming)
     (Hinv : renamings_inv r r')
     (st   : state Z) : rename_state r (rename_state r' st) = st.
-  Proof. admit. Admitted.
-      
+  Proof. unfold renamings_inv in Hinv. induction st.
+  - simpl. reflexivity.
+  - replace (a :: st) with ([a] ++ st).
+    + rewrite rename_state_dist. rewrite rename_state_dist.
+      rewrite IHst. destruct a. rewrite rename_state_id. rewrite rename_state_id. rewrite Hinv. reflexivity.
+    + auto.
+  Qed.
+
   Lemma bijective_injective (f : id -> id) (BH : Bijective f) : Injective f.
-  Proof. admit. Admitted.
-  
+  Proof. unfold Bijective in BH. destruct BH as [g [H1 H2]]. unfold Injective.
+  intros. assert (g (f x) = g (f y)).
+    { f_equal. apply H. }
+  rewrite H1 in H0. rewrite H1 in H0. apply H0.
+  Qed.
+
+  (* Silly statement, but it's convenient to have it as a separate lemma *)
+  Lemma nat_eval_any_state (n n': Z) (s1 s2: state Z):
+    [|Nat n|] s1 => n' <-> [|Nat n|] s2 => n'.
+  Proof. split.
+  - intros. inversion H. subst. constructor.
+  - intros. inversion H. subst. constructor.
+  Qed.
+
+  Lemma rename_id_inj (r: renaming) (i1 i2: id) (EQ: rename_id r i1 = rename_id r i2):
+    i1 = i2.
+  Proof. destruct r as [f b]. simpl in EQ. apply bijective_injective in b. apply b. apply EQ. Qed.
+
+  Lemma rename_id_state_tail (r: renaming) (s: state Z) (i i0: id) (z z0: Z) (NEQ: i <> i0):
+    (rename_state r ((i0, z0) :: s)) / (rename_id r i) => z <-> (rename_state r s) / (rename_id r i) => z.
+  Proof. replace ((i0, z0) :: s) with ([(i0, z0)] ++ s) by auto.
+  rewrite rename_state_dist. rewrite rename_state_id. simpl.
+  split; intros H; inversion H; subst;
+  try (apply rename_id_inj in H4; subst; congruence);
+  try apply H6;
+  constructor;
+  ((intros NEQ2; apply rename_id_inj in NEQ2) + constructor);
+  congruence.
+  Qed.
+
+  Lemma rename_id_state (r: renaming) (s: state Z) (i: id) (z: Z):
+    s / i => z <-> (rename_state r s) / (rename_id r i) => z.
+  Proof. induction s.
+  - simpl. split; intros H; apply st_not_binds_empty in H; destruct H.
+  - destruct a. destruct (id_eq_dec i i0).
+    + subst. replace ((i0, z0) :: s) with ([(i0, z0)] ++ s) by auto.
+      rewrite rename_state_dist. rewrite rename_state_id. simpl. split;
+      intros H; inversion_clear H;
+      try constructor;
+      congruence.
+    + split.
+      * intros. rewrite rename_id_state_tail by congruence. rewrite <- IHs. inversion H; subst; congruence.
+      * intros. rewrite rename_id_state_tail in H by congruence. constructor.
+        { congruence. }
+        { rewrite IHs. apply H. }
+  Qed.
+
   Lemma eval_renaming_invariance (e : expr) (st : state Z) (z : Z) (r: renaming) :
     [| e |] st => z <-> [| rename_expr r e |] (rename_state r st) => z.
-  Proof. admit. Admitted.
-    
+  Proof. generalize dependent z. induction e.
+  - intros. simpl. induction st.
+    + reflexivity.
+    + apply nat_eval_any_state.
+  - intros. induction st.
+    + simpl. split; intros; inversion H; subst; inversion VAR.
+    + split;
+      intros; constructor; replace (a :: st) with ([a] ++ st) by auto;
+      replace (a :: st) with ([a] ++ st) in H by auto.
+      * rewrite <- rename_id_state. inversion_clear H. apply VAR.
+      * inversion_clear H. rewrite <- rename_id_state in VAR. apply VAR.
+  - simpl. split;
+    intros; inversion_clear H;
+    econstructor; ((apply IHe1; apply VALA) + (apply IHe2; apply VALB) + congruence).
+  Qed.
+
 End Renaming.
